theory/lang/regmachine.v
@@ -1,8 +1,9 @@
+From RelationAlgebra Require Import lattice monoid rel kat kat_tac kleene.
 From mathcomp Require Import ssreflect ssrfun ssrbool ssrnat seq.
-From mathcomp Require Import eqtype choice finfun finmap tuple.
+From mathcomp Require Import eqtype choice finfun finmap tuple order.
 From monae Require Import hierarchy monad_model.
 From eventstruct Require Import utils eventstructure inhtype.
-From eventstruct Require Import transitionsystem ident.
+From eventstruct Require Import transitionsystem ident rewriting_system.
 
 (******************************************************************************)
 (* Here we want to define big-step semaintics of simple register machine in   *)
@@ -55,8 +56,6 @@ Open Scope fmap_scope.
 Open Scope do_notation.
 Open Scope exec_eventstruct_scope.
 
-Import Label.Syntax.
-
 Local Notation M := ModelMonad.ListMonad.t.
 
 Context {disp} {E : identType disp} {Val : inhType}.
@@ -79,11 +78,28 @@ Inductive instr :=
 | CJmp     of Reg & nat 
 | Stop.
 
-Definition seqprog := seq instr.
+Definition eq_instr st st' :=
+  match st, st' with
+  | WriteReg x r, WriteReg y s => [&& x == y & r == s]
+  | ReadLoc  x l, ReadLoc  y m => [&& x == y & l == m]
+  | WriteLoc x l, WriteLoc y m => [&& x == y & l == m]
+  | CJmp     r n, CJmp     s m => [&& r == s & n == m]
+  | Stop        , Stop         => true
+  | _           , _            => false
+  end.
 
-Definition empty_prog : seqprog := [::].
+Lemma eqinstrP : Equality.axiom eq_instr.
+Proof.
+  case=> [??|??|??|??|][]*/=; (try by constructor); 
+  by apply/(iffP andP)=> [[/eqP->/eqP]->|[->->]].
+Qed.
 
-Definition parprog := seq seqprog.
+Canonical instr_eqMixin := EqMixin eqinstrP.
+Canonical instr_eqType  := Eval hnf in EqType instr instr_eqMixin.
+
+Definition prog := seq instr.
+
+Definition empty_prog : prog := [::].
 
 Record thrd_state := Thrd_state {
   ip     : nat;
@@ -105,53 +121,73 @@ Canonical thrd_state_eqType :=
 Definition init_state : thrd_state := {| ip := 0; regmap := [fsfun with inh] |}.
 
 Record config := Config {
-  evstr    : cexec_event_struct;
-  trhdmap  :> {fsfun E -> (thrd_state * nat)%type with (init_state, 0)}
+  evstr     :> exec_event_struct;
+  thrdmap   : {fsfun E -> thrd_state with init_state}
 }.
 
-Notation inth := (nth Stop).
+Definition eq_config c c' :=
+  (evstr c == evstr c') && (thrdmap c == thrdmap c').
 
-Definition thrd_sem (pgm : seqprog) (st : thrd_state) :
-  (option (@Lab unit Val) * (Val -> thrd_state))%type :=
+Lemma eqconfigP : Equality.axiom eq_config.
+Proof.
+  by move=> [??] [??]; apply: (iffP andP)=> /= [[/eqP + /eqP]|[]] => <-<-.
+Qed.
+
+Canonical config_eqMixin := EqMixin eqconfigP.
+Canonical config_eqType  := Eval hnf in EqType config config_eqMixin.
+
+Coercion thrdmap : config >-> fsfun.
+
+Definition thrd_prositions := 
+  let fix thrd_pos s n pgm :=
+    match pgm with
+    | [::]        => s
+    | ins :: pgm => 
+      if ins == Stop then
+        thrd_pos (n :: s) n.+1 pgm
+      else thrd_pos s n pgm
+    end in
+      thrd_pos [::] 1%N.
+
+Definition prog_sem (pgm : prog) (st : thrd_state) :
+  seq (@Lab unit Val * (Val -> thrd_state)) :=
   let: {| ip := ip; regmap := rmap |} := st in
-  if ip == 0 then
-    (Some ThreadStart, fun=> {| ip := 1; regmap := rmap |})
+  if ip == 0%N then do 
+    ip <- thrd_prositions pgm : M _;
+                      [:: (ThreadStart,
+                      fun _ => {| ip     := ip.+1;
+                                  regmap := rmap |})]
   else
-    match inth pgm ip.-1 with
-    | WriteReg v r => (None,
+    match nth Stop pgm ip.-1 with
+    | WriteReg v r => [:: (Eps,
                       fun _ => {| ip     := ip.+1;
-                                  regmap := [fsfun rmap with r |-> v] |})
-    | ReadLoc  r x => (Some (Read x __),
+                                  regmap := [fsfun rmap with r |-> v] |})]
+    | ReadLoc  r x => [:: (Read x __,
                       fun v => {| ip     := ip.+1;
-                                  regmap := [fsfun rmap with r |-> v] |})
-    | WriteLoc v x => (Some (Write x v),
+                                  regmap := [fsfun rmap with r |-> v] |})]
+    | WriteLoc v x => [:: (Write x v,
                       fun _ => {| ip     := ip.+1;
-                                  regmap := rmap |})
-    | CJmp     r n => (None,
+                                  regmap := rmap |})]
+    | CJmp     r n => [:: (Eps,
                       fun _ => {| ip     := if rmap r != inh then n.+1 else ip.+1;
-                                  regmap := rmap |} )
-    | Stop         => (None, fun=> st)
+                                  regmap := rmap |} )]
+    | Stop         => [:: (Eps, fun=> st)]
     end.
 
-Definition ltr_thrd_sem (l : option (@Lab Val Val)) pgm st1 st2 : bool :=
-  match thrd_sem pgm st1, l with
-  | (Some (Write x v), st), Some (Write y u) => [&& x == y, v == u & st inh == st2]
-  | (Some (Read  x _), st), Some (Read  y u) => (x == y) && (st u == st2)
-  | (Some ThreadStart, st), Some ThreadStart => st inh == st2
-  | (None            , st), None             => st inh == st2
-  | _, _                                     => false
-  end.
+Section AddHole.
 
-Variable (es : cexec_event_struct).
-Notation ffpo     := (fpo es).
+Variable (es : exec_event_struct).
+Notation ffpred   := (fpo es).
 Notation ffrf     := (frf es).
 Notation fresh_id := (fresh_seq (dom es)).
 
-(* Arguments add_label_of_Nread {_ _ _ _} _ {_}. *)
+Arguments add_label_nread {_ _ _ _ _} _.
 
-Lemma ws_mem x w : 
+Lemma ws_mem x w :
   w \in [events of es | is_write & with_loc x] -> w \in dom es.
 Proof. by rewrite ?inE mem_filter => /andP[?->]. Qed.
+
+Import Label.Syntax. 
 
 Lemma ws_wpred x w :
   w \in [events of es | is_write & with_loc x] ->
@@ -165,77 +201,510 @@ Proof.
   by rewrite !eq_refl.
 Qed.
 
-Definition es_seq x {pr} : (seq (exec_event_struct * E)) :=
+Definition es_seq x pr : (seq (exec_event_struct * Val)) :=
   if pr \in dom es =P true is ReflectT pr_mem then
     [seq
       let: wr       := sval w in
       let: w_in     := valP w in
       let: read_lab := Read x (odflt inh (value es wr)) in
       (
-        add_new_event
+        add_event
           {| add_lb            := read_lab;
+             add_lb_init       := erefl;
              add_pred_in_dom   := pr_mem;
              add_write_in_dom  := ws_mem   w_in;
              add_write_consist := ws_wpred w_in; |},
-        wr
+          (odflt inh (value es wr))
       ) | w <- seq_in [events of es | is_write & with_loc x]]
   else [::].
 
-Definition ces_seq_aux x pr := 
-  [seq estr_w <- @es_seq x pr | 
-    let: (estr, w) := estr_w in
-   ~~ (cf estr fresh_id w)].
-
-Lemma mem_ces_seq_aux x pr ces: 
-  ces \in (@ces_seq_aux x pr) -> dom_consistency ces.1.
-Proof.
-  case: ces => ces w; rewrite mem_filter /= /es_seq => /andP[?].
-  case: eqP=> // ? /mapP[?? [/[dup] C -> ws]].
-  move: C. rewrite /add_new_event; case: ifP=> _ C; first by case: es.
-  apply/consist_add_event=> /=; first by case: es.
-  by rewrite -C -ws.
-Qed.
-
-Definition ces_seq x pr := 
-  [seq 
-    let: ces_w    := sval ces_w_mem in
-    let: (ces, w) := ces_w in
-    let: ces_mem  := valP ces_w_mem in 
-    (Consist _ (mem_ces_seq_aux ces_mem), odflt inh (value es w)) | 
-    ces_w_mem <- seq_in (@ces_seq_aux x pr)].
-
-Arguments consist_new_nread {_ _ _}.
-
-Definition add_hole
-  (l : @Lab unit Val) pr :
-  seq (cexec_event_struct * Val) :=
+Definition add_hole (l : @Lab unit Val) pr : 
+  seq (exec_event_struct * Val) :=
   if pr \in dom es =P true is ReflectT pr_mem then
     match l with
-    | Write x v => 
-      [:: (Consist _ (consist_new_nread es pr (Write x v) pr_mem erefl), v)]  
+    | Read  x _   => es_seq x pr
+    | Write x v   =>
+      [:: (add_event (add_label_nread (Write x v) pr_mem erefl erefl), v)]
     | ThreadStart =>
-      [:: (Consist _ (consist_new_nread es pr ThreadStart pr_mem erefl), inh)]
-    | Read x __ => ces_seq x pr
-    | _         => [::]
+      [:: (add_event (add_label_nread ThreadStart pr_mem erefl erefl), inh)]
+    | ThreadEnd   =>
+      [:: (add_event (add_label_nread ThreadEnd pr_mem erefl erefl), inh)]
+    | _           => [::]
     end
   else [::].
 
-Variable prog : parprog.
+End AddHole.
 
-Definition fresh_tid (c : config) := 
-  foldr maxn 0 [seq (snd x).+1 | x <- fgraph (fmap_of_fsfun c)].
+Variable pgm : prog.
 
 Definition eval_step (c : config) pr : seq config := 
-  let: Config es tmap := c in
-  let: (conf, tid)    := tmap pr in
-  let: tid            := if pr \in dom es then tid else fresh_tid c in
-  let: (l, cont_st)   := thrd_sem (nth empty_prog prog tid) conf in
-    if l is Some l then do 
-      ev <- add_hole l pr : M _;
-      let '(e, v) := ev in
-        [:: Config e  [fsfun c with fresh_id |-> (cont_st v, tid)]]
-    else
-      [:: Config es [fsfun c with pr |-> (cont_st inh, tid)]].
+  if pr \in dom c then 
+    do prg_st <- prog_sem pgm (c pr) : M _;
+    let: (l, cont_st) := prg_st in
+      if l != Eps then do 
+        ev <- add_hole c l pr : M _;
+        let '(e, v) := ev in
+          [:: Config e [fsfun c with fresh_seq (dom c) |-> cont_st v]]
+      else
+        [:: Config c [fsfun c with pr |-> cont_st inh]]
+  else [::].
 
 End RegMachine.
+
+Notation fresh_id1  es := (fresh_seq (dom es)).
+Notation fresh_id2 es := (fresh_seq (fresh_seq (dom es) :: dom es)).
+
+Module AddHole.
+
+Section AddHoleConfl.
+
+Open Scope fmap_scope.
+Open Scope do_notation.
+Open Scope exec_eventstruct_scope.
+
+Context {disp} {E : identType disp} {Val : inhType}.
+
+(*Notation n := (@n val).*)
+Notation exec_event_struct := (fin_exec_event_struct E Val).
+Notation cexec_event_struct := (cexec_event_struct E Val).
+
+Definition ltr (l : (@Lab unit Val) * E * Val) es es'
+  := (es', l.2) \in add_hole es l.1.1 l.1.2.
+
+Definition tr es es' := exists (l : (@Lab unit Val)) (pr : E) (v : Val),
+   (es', v) \in add_hole es l pr.
+
+Notation "e1 '~(' l ',' pr ',' v ')~>' e2" := (ltr (l, pr, v) e1 e2) (at level 20).
+
+Lemma exlab_tr : tr ≡ exlab ltr.
+Proof.
+  move=> ??; split=> [[l [pr [v]]]|[[[l pr v]]]] ?; 
+  by [exists (l, pr, v)| exists l, pr, v].
+Qed.
+
+Notation "e1 '~>' e2" := (tr e1 e2).
+
+Definition fill_hole (l : @Lab unit Val) (v : Val) := 
+  match l with
+  | Read x _    => Read x v
+  | Write x v   => Write x v
+  | ThreadStart => ThreadStart
+  | ThreadEnd   => ThreadEnd
+  | Eps         => Eps
+  | Init        => Init
+  end.
+
+Definition mk_hole (l : @Lab Val Val) := 
+  match l with
+  | Read x v    => Read x tt
+  | Write x v   => Write x v
+  | ThreadStart => ThreadStart
+  | ThreadEnd   => ThreadEnd
+  | Eps         => Eps
+  | Init        => Init
+  end.
+
+Lemma fill_mk_hole l : fill_hole (mk_hole l) (odflt inh (Label.value l)) = l.
+Proof. by case: l. Qed.
+
+Import Label.Syntax.
+
+Arguments add_nread_synch {_ _ _ _} _.
+
+Lemma ltrP {es1 es2 la pr v} :
+  reflect
+  (exists (l : edescr E Lab),
+  [/\ AddEvent.ltr l es1 es2,
+      fpo_prj l                           = pr,
+      fill_hole la v                      = lab_prj l &
+      odflt inh (Label.value (lab_prj l)) = v])
+  (es1 ~(la, pr, v)~> es2).
+Proof.
+  apply: (iffP idP).
+  - rewrite /ltr /= /add_hole; case: eqP=> // p.
+    case: la=> //=.
+    - move=> l ?; rewrite /es_seq; case: eqP=> // ?.
+      rewrite seq_inE=> /mapP=> [[[/= e p' I [-> El]]]].
+      exists (mk_edescr (Read l v) pr e); split=> //.
+      apply/AddEvent.ltr_add=> /=; by rewrite El.
+    1-3: move=>>; rewrite ?inE=> /eqP [-><-];
+      eexists (mk_edescr _ pr \i0); split=> //;
+      exact/AddEvent.ltr_add.
+  rewrite /ltr /==> [[[/= l p w [+ <-]]]].
+  move=> /[dup][[[/= ??? + ??? _ []]]]; move=> /[swap]{1 2}<- ni ??.
+  move=> /[dup] /AddEvent.ltr_po /= Ip /[swap]++/[swap].
+  rewrite /add_hole; case: eqP=> [?|]; last by rewrite Ip.
+  case: la=> /=.
+  - move=> la _ <- /= _ [[l' p' w' +++++ [el ep ew]]].
+    case: _ / ep el ew; (do ? case: _ /)=> ?? wd wc ->.
+    rewrite /es_seq; case: eqP=> [?|]; last by rewrite Ip.
+    apply/mapP.
+    have I: w \in [events of es1 | is_write & with_loc la].
+    - move: wc; rewrite mem_filter wd /= /is_write /= /with_loc /= /loc /=.
+    case: (lab es1 w)=> //= > /andP[/eqP->]; by rewrite eq_refl.
+    exists (exist _ w I); first by rewrite seq_in_mem.
+    apply/congr2=> /=; first (apply/congr1/of_add_label_inj=> /=);
+    by rewrite /value /= (synch_val _ _ _ _ wc).
+  1-3: move=>> <- /=-> [al -> Eal]; rewrite ?inE; apply/eqP;
+  congr (_, _); apply/congr1/of_add_label_inj=> /=;
+  rewrite -Eal; apply/congr1; case: al Eal=> /= ?? aw ??? /[swap][[<-?->]];
+  rewrite /(_ \>> _); case: (lab es1 aw =P Init); last (by case: (lab _ _));
+  by move/lab_Init.
+  all: move=> E'; by rewrite E' eq_refl ?andbF in ni.
+Qed.
+
+Definition eqv := (@AddEvent.eqv disp E Val).
+
+Lemma iso_swap l1 pr1 v1 l2 pr2 v2 es1 es2 es3:
+  es1 ~(l1, pr1, v1)~> es2 ->
+  es1 ~(l2, pr2, v2)~> es3 ->
+  exists es4 es4',
+    [/\ es2 ~(l2, pr2, v2)~> es4,
+        es3 ~(l1, pr1, v1)~> es4' &
+        AddEvent.is_iso (swap id (fresh_id1 es1) (fresh_id2 es1)) es4 es4'].
+Proof.
+  case/ltrP=> la1 [/AddEvent.iso_swap L ??? /ltrP[la2 [/L]]].
+  case=> es4 [es4' [l*]]; exists es4, es4'.
+  split=> //; apply/ltrP; by [exists la2| exists la1].
+Qed.
+
+Lemma comm_ltr l1 l2 : eqv_diamond_commute (ltr l1) (ltr l2) eqv.
+Proof.
+  move=> es1 ?? /iso_swap/[apply][[es4 [es4' [*]]]].
+  by exists es4, es4'; split=> //; exists (swap id (fresh_id1 es1) (fresh_id2 es1)).
+Qed.
+
+Lemma iso_swap_eqv l1 pr1 v1 f g es1 es2 es3: 
+  let: h := swap f (fresh_id1 es1) (g (fresh_id1 es3)) in
+  es1 ~(l1, pr1, v1)~> es2 ->
+  AddEvent.is_iso f es1 es3 -> 
+  cancel g f -> 
+  exists es4,
+    [/\ es3 ~(l1, h pr1, v1)~> es4 &
+        AddEvent.is_iso h es2 es4].
+Proof.
+  case/ltrP=> al [/AddEvent.iso_swap_eqv L H1 H2 H3 {L}/L/[apply]].
+  set h := (swap f (fresh_id1 es1) (g (fresh_id1 es3))).
+  case=> es4 [[al' -> Le ?]]; exists (add_event al'); split=> //.
+  apply/ltrP; exists (edescr_map h al); split=> //.
+  - by exists al'.
+  - rewrite Le; by case: (al') (al) H1 Le=> /= > I ??? [/=> <- [?]].
+  1,2: by move: H2 H3; case: (al).
+Qed.
+
+Lemma comm_eqv_tr :
+  diamond_commute eqv tr.
+Proof.
+  move=> es1 es2 ?; rewrite (exlab_tr _ _)=> [[f /[dup] [[_ [g ? c I]]]]].
+  set h := swap f (fresh_id1 es1) (g (fresh_id1 es2)).
+  case=> [[[l pr v /iso_swap_eqv/(_ I c)[es4 [??]]]]].
+  exists es4; last by exists h.
+  by rewrite (exlab_tr _ _); exists (l, h pr, v).
+Qed.
+
+Lemma ltr_fresh es1 es2 l v pr :
+  es1 ~(l, pr, v)~> es2 -> fresh_id2 es1 = fresh_id1 es2.
+Proof. by move/ltrP=> [? [[? ->]]]. Qed.
+
+Lemma ltr_dom es1 es2 l v pr :
+  es1 ~(l, pr, v)~> es2 -> pr \in dom es1.
+Proof. by rewrite /ltr /add_hole; case: eqP. Qed.
+
+Lemma ltr_dom2 es1 es2 l v pr :
+  es1 ~(l, pr, v)~> es2 -> dom es2 = fresh_id1 es1 :: dom es1.
+Proof. by move/ltrP=> [? [[? ->]]]. Qed.
+
+End AddHoleConfl.
+
+End AddHole.
+
+Module Prog.
+
+Section ProgConfl.
+
+Open Scope fmap_scope.
+Open Scope do_notation.
+Open Scope exec_eventstruct_scope.
+
+Context {Val : inhType}.
+
+Variable pgm : prog (Val := Val).
+
+Definition ltr (l : (@Lab unit Val) * Val) st st' := 
+  (l.1, st') \in [seq (x.1, x.2 l.2) | x <- prog_sem pgm st].
+
+Notation "e1 '~(' l ',' v ')~>' e2" := (ltr (l, v) e1 e2) (at level 20).
+
+Lemma Eps_det st st1 st2 v u l: 
+  st ~(Eps, v)~> st1 ->
+  st ~(l  , u)~> st2 ->
+  ((st1 = st2) * (l = Eps))%type.
+Proof.
+  case: st=> /=; rewrite /ltr /==> ??; case: ifP=> //. 
+  - move=> ? L; exfalso; move: L; by elim: (thrd_prositions pgm).
+  by case: (nth Stop pgm _.-1)=> //= > ?; rewrite ?inE=> /eqP[-> /eqP [->]].
+Qed.
+
+End ProgConfl.
+
+End Prog.
+
+Module RegMachine.
+
+Section RegMachineConfl.
+
+Import Order.LTheory.
+
+Open Scope fmap_scope.
+Open Scope do_notation.
+Open Scope exec_eventstruct_scope.
+Open Scope order_scope.
+
+Local Notation M := ModelMonad.ListMonad.t.
+
+Context {disp} {E : identType disp} {Val : inhType}.
+
+(*Notation n := (@n val).*)
+Notation exec_event_struct := (fin_exec_event_struct E Val).
+Notation cexec_event_struct := (cexec_event_struct E Val).
+
+Variable pgm : prog (Val := Val).
+
+Implicit Type c : @config disp E Val.
+
+Notation eval_step := (eval_step pgm (disp := disp) (E := E)).
+Notation Progltr := (Prog.ltr pgm).
+
+Definition ltr pr (c c' : config) := c' \in eval_step c pr.
+
+Notation "c1 '~(' pr ')~>' c2" := (ltr pr c1 c2) (at level 20).
+
+Definition tr := exlab ltr.
+
+Definition is_iso (f : E -> E) c c' := 
+  AddEvent.is_iso f c c' /\ {in dom c, c =1 c' \o f}.
+
+Lemma is_iso_id c : is_iso id c c.
+Proof. split=> //; exact/AddEvent.is_iso_id. Qed.
+
+Definition eqv := exlab is_iso.
+
+Lemma eqvcc c : eqv c c.
+Proof. exists id; exact/is_iso_id. Qed.
+
+Lemma eqv_symm : Symmetric eqv.
+Proof.
+  move=> ?? [f [/[dup][[? [g /[dup] c1 /AddEvent.is_iso_can L /[dup]]]]]].
+  move=> {L}/L L c2 /[dup] /L ? I D; exists g; split=> // x.
+  rewrite -(AddEvent.iso_dom I) -{1}[x]c2 (mem_map (can_inj c1))=> /D /=.
+  by rewrite c2.
+Qed.
+
+Lemma eqv_evstr c c': eqv c c' -> AddEvent.eqv c c'.
+Proof. case=> f []; by exists f. Qed.
+
+Definition silent_ltr pr c c' := 
+  [/\ Progltr (Eps, inh) (c pr) (c' pr),
+      pr \in dom c,
+      [fsfun c with pr |-> c' pr] = c' &
+      c = c' :> exec_event_struct].
+
+Lemma silent_det c c1 c2 pr : 
+  silent_ltr pr c c1 ->
+  silent_ltr pr c c2 ->
+  c1 = c2.
+Proof.
+  case=> /Prog.Eps_det L +++ [{L}/L<-].
+  case: c1 c2=> /= e1 t1 [/= e2 t2 ? <-<- ? <-<-].
+  by rewrite fsfun_with.
+Qed.
+
+Definition non_silent_ltr pr c c' := 
+  exists l v, 
+  [/\ Progltr (l, v) (c pr) (c' (fresh_id1 c)),
+      l != Eps,
+      [fsfun c with fresh_id1 c |-> c' (fresh_id1 c)] = c' &
+      AddHole.ltr (l, pr, v) c c'].
+
+Lemma non_silent_dom pr c c' : 
+  non_silent_ltr pr c c' -> pr \in dom c.
+Proof. by case=> ? [? [??? /AddHole.ltr_dom]]. Qed.
+
+Lemma silent_dom pr c c' : 
+  silent_ltr pr c c' -> pr \in dom c.
+Proof. by case. Qed.
+
+Lemma ltrP c c' pr : 
+  reflect (silent_ltr pr c c' \/ non_silent_ltr pr c c')
+    (c ~(pr)~> c').
+Proof.
+  apply: (iffP idP); rewrite /ltr /eval_step.
+  - case: ifP=> D //.
+    have: forall v l st, 
+      (l, st) \in [seq (x.1, x.2 v) | x <- prog_sem pgm (c pr)] ->
+      Progltr (l, v) (c pr) st by [].
+    elim: (prog_sem pgm (c pr))=> //=.
+    move=> [l cont /= conts] IHp H; rewrite do_cons mem_cat=> /orP[].
+    - move: H; case: (l =P Eps)=> /= [->/(_ inh Eps (cont inh) (mem_head _ _))|].
+      - rewrite ?inE=> P /eqP->; left.
+        split=> //=; by rewrite fsfun_with.
+      move=> /eqP ? H /do_mem[[es v ?]].
+      rewrite ?inE=> /eqP->; right; exists l, v.
+      split=> //=; rewrite ?fsfun_with //; exact/H/mem_head.
+    by apply/IHp=> ??? I; apply/H; rewrite ?inE I.
+  have H: forall v l st, Progltr (l, v) (c pr) st ->
+    (l, st) \in [seq (x.1, x.2 v) | x <- prog_sem pgm (c pr)] by [].
+  case: ifP=> [?|/[swap][[/silent_dom|/non_silent_dom]]->] //.
+  case=> [|[l[v]]][]; rewrite /Prog.ltr /=; 
+  elim: (prog_sem pgm (c pr))=> //= [][la cont ? /=];
+  rewrite do_cons mem_cat; move=> IHp.
+  - rewrite ?inE=> /orP[/eqP|/IHp/[apply]/[apply]/[apply]->//].
+    case=><-->; rewrite eq_refl /= ?inE /eq_op /= /eq_config /==>?<-<-;
+    by rewrite ?eq_refl.
+  rewrite ?inE=> /orP[/eqP[->+->]|/IHp/[apply]/[apply]/[apply]->//].
+  move=> E1 E2 ?. apply/orP; left; apply/do_mem; exists (evstr c', v)=> //.
+  by rewrite ?inE /eq_op /= /eq_config /= -E1 E2 ?eq_refl. 
+Qed.
+
+Lemma rltrP c c' pr : 
+  ((1 + (silent_ltr pr : hrel _ _))%ra c c' \/
+   (1 + (non_silent_ltr pr : hrel _ _))%ra c c') <->
+  ((1 + (ltr pr : hrel _ _))%ra c c').
+Proof.
+  split=> [[|][->|]|[->|/ltrP[]]] *; try by (right + left).
+  - by right; apply/ltrP; left.
+  - by right; apply/ltrP; right.
+  all: by do ? (left + right).
+Qed.
+
+Lemma comm_nnltr {pr1 pr2}:
+  eqv_rdiamond_commute (non_silent_ltr pr1) (non_silent_ltr pr2) eqv.
+Proof.
+  apply/diamond_rdiamod.
+  move=> c1 c2 c3 [l [v [?? E1 /[dup]/AddHole.ltr_fresh fr ]]].
+  move=> /[dup]/AddHole.ltr_dom I1 /AddHole.iso_swap L [m [u [?? E2]]].
+  move=> /[dup]/AddHole.ltr_fresh fr' /[dup] /AddHole.ltr_dom I2 {L}/L.
+  case=> es4 [es4' [???]].
+  have N: (fresh_id1 c1) == (fresh_id2 c1) = false.
+  - by apply/negbTE/eqP=> /(@fresh_iter _ _ 1 2).
+  exists (Config es4  [fsfun c2 with fresh_id2 c1 |-> c3 (fresh_id1 c1)]),
+         (Config es4' [fsfun c3 with fresh_id2 c1 |-> c2 (fresh_id1 c1)]).
+  split=> /=.
+  - exists m, u; split=> //=; rewrite -?fr fsfun_with //.
+    rewrite -E1 fsfun_withE (lt_eqF (fresh_seq_lt dom_sorted I2)) //.
+  - exists l, v; split=> //=; rewrite -?fr' ?fsfun_with //.
+    rewrite -E2 fsfun_withE (lt_eqF (fresh_seq_lt dom_sorted I1)) //.
+  exists (swap id (fresh_id1 c1) (fresh_id2 c1)); split=> //= x.
+  rewrite -E1 -E2 /=; rewrite fsfun_withE; case: ifP=> [/eqP->|N1].
+  - rewrite swap2 ?fsfun_withE eq_refl N //.
+  rewrite fsfun_withE; case: ifP=> [/eqP->|N2].
+  - by rewrite swap1 ?fsfun_with.
+  by rewrite -swap_not_eq // ?fsfun_withE ?(N1, N2).
+Qed.
+
+Lemma comm_ssltr {pr1 pr2}: 
+  eqv_rdiamond_commute (silent_ltr pr1) (silent_ltr pr2) eqv.
+Proof.
+  move=> c1 c2 c3.
+  case: (pr1 =P pr2)=> [-> /silent_det/[apply]->|/eqP/negbTE N].
+  - exists c3, c3; split; last (exact/eqvcc); by left.
+  case=> [? D1 C1 E1 [? D2 C2 E2]].
+  exists (Config c2 [fsfun c2 with pr2 |-> c3 pr2]),
+         (Config c3 [fsfun c3 with pr1 |-> c2 pr1]).
+  split; rewrite -1?C1 -1?C2 ?fsfun_with.
+  - right; split=> //=; rewrite -?E1 // fsfun_with //.
+    - rewrite -C1 fsfun_withE eq_sym N //.
+    by rewrite -{1}C1.
+  - right; split=> //=; rewrite -?E2 // fsfun_with //.
+    - rewrite -C2 fsfun_withE N //.
+    by rewrite -{1}C2.
+  exists id; rewrite -E1 -E2; split=> /=; first exact/AddEvent.is_iso_id.
+  move=> ?; rewrite /= ?fsfun_withE; case: ifP=> [/eqP->|//].
+  by rewrite eq_sym N.
+Qed.
+
+Lemma comm_nsltr {pr1 pr2}: 
+  eqv_rdiamond_commute (non_silent_ltr pr1) (silent_ltr pr2) eqv.
+Proof.
+  apply/diamond_rdiamod.
+  move=> c1 c2 c3 [l [v [p1 N C1 L [p2 I2 C2 Ec]]]].
+  do ? exists (Config c2 
+          [fsfun c1 with pr2          |-> c3 pr2,
+                         fresh_id1 c1 |-> c2 (fresh_id1 c1)]).
+  split=> //=; last exact/eqvcc.
+  - split=> //=. 
+    - rewrite -{1}C1 ?fsfun_withE eq_refl; case: ifP=> //.
+      by rewrite (lt_eqF (fresh_seq_lt dom_sorted I2)).
+    - by rewrite (AddHole.ltr_dom2 L) ?inE I2.
+    by rewrite fsfun_with -{1}C1.
+  exists l, v; split=> //=; rewrite -?Ec // ?fsfun_withE.
+  - rewrite eq_refl eq_sym (lt_eqF (fresh_seq_lt dom_sorted I2)).
+    rewrite -C2 fsfun_withE.
+    by case: ifP p2 p1 N=> // /eqP-> /Prog.Eps_det/[apply]->.
+  rewrite eq_refl eq_sym ((lt_eqF (fresh_seq_lt dom_sorted I2))).
+  rewrite -{1}C2; apply/fsfunP=> ?; rewrite ?fsfun_withE.
+  case: ifP=> // /eqP->. 
+  by rewrite eq_sym ((lt_eqF (fresh_seq_lt dom_sorted I2))).
+Qed.
+
+Lemma comm_ltr pr1 pr2 : eqv_rdiamond_commute (ltr pr1) (ltr pr2) eqv.
+Proof.
+  move=> ??? /ltrP[] t1 /ltrP[] t2.
+  - case: (comm_ssltr t1 t2)=> s4 [s4' [*]].
+  2: case: ((comm_nsltr t2 t1))=> s4' [s4 [?? /eqv_symm ?]]. 
+  3: case: (comm_nsltr t1 t2)=> s4 [s4' [*]].
+  4: case: (comm_nnltr t1 t2)=> s4 [s4' [*]].
+  all: exists s4, s4'; split=> //; apply/rltrP; by (left + right). 
+Qed.
+
+Lemma comm_tr_eqv : diamond_commute eqv tr.
+Proof.
+  move=> c1 c3 c2 /[swap][] [pr T].
+  have In : pr \in dom c1 by move: T; rewrite /ltr /eval_step; case: ifP.
+  case/ltrP: T=> [[?? T C [f [/[dup] L [_ b] C1]]]|].
+  - exists (Config c3 [fsfun c3 with f pr |-> c2 pr]).
+  - exists (f pr); apply/ltrP; left; split=> //=.
+    - move: (C1 _ In)=> /=<-. by rewrite fsfun_with.
+    - rewrite -(AddEvent.iso_dom L) mem_map //; exact/bij_inj.
+      by rewrite fsfun_with.
+    exists f; split=> //= [|?]; rewrite -C // => D.
+    rewrite /= -T ?fsfun_withE eq_refl (bij_eq b).
+    by move: (C1 _ D)=> /=->.
+  case=> l [v [?? E1 /[dup] T /AddHole.iso_swap_eqv L]].
+  case=> [f /[dup][[/[dup] Is[? /[dup] bf [g c' c _]]]]] [] /L/(_ c)[es4 []].
+  set h := swap f (fresh_id1 c1) (g (fresh_id1 c3))=> ?? /[dup]C /(_ pr) /= Eq.
+  exists (Config es4 [fsfun c3 with fresh_id1 c3 |-> c2 (fresh_id1 c1)]). 
+  - exists (h pr); apply/ltrP; right; exists l, v; split=> //=.
+    - rewrite fsfun_with /h -swap_not_eq -?Eq //; apply/eqP; move: In=> /[swap].
+      - by move->=>/(negP (fresh_seq_notin dom_sorted)).
+      move->; rewrite -[dom c1](mapK c') mem_map; last exact/can_inj.
+      by rewrite (AddEvent.iso_dom Is)=> /(negP (fresh_seq_notin dom_sorted)).
+    by rewrite fsfun_with.
+  exists h; split=> // x /=; rewrite -{1}E1 /h /swap fsfun_withE.
+  case: ifP=> [|]; first rewrite c fsfun_with //.
+  have D: dom c2 = fresh_id1 c1 :: dom c1 by apply/(AddHole.ltr_dom2 T).
+  case: ifP=> [/eqP->|N1]; rewrite D ?inE=>-> /=.
+  - rewrite -[dom c1](mapK c') mem_map; last exact/can_inj.
+    by rewrite (AddEvent.iso_dom Is)=> /(negP (fresh_seq_notin dom_sorted)).
+  by move/C=> /=->; rewrite fsfun_withE -[fresh_id1 _]c (bij_eq bf) N1.
+Qed.
+
+Theorem ltr_confl : eqv_rconfluent tr eqv.
+Proof.
+  apply/(eqv_comm_union _ _ _ eqv_symm _ comm_ltr comm_tr_eqv).
+  - move=> ??? [f [L1 D1 [g [L2 D2]]]]; exists (g \o f); split.
+    - exact/(AddEvent.is_iso_comp L1 L2).
+    move=> ? /[dup] D /D1 /=->; apply/D2.
+    rewrite -(AddEvent.iso_dom L1) mem_map //; exact/bij_inj/(L1.2).
+  move=> ??->; exact/eqvcc.
+Qed.
+
+End RegMachineConfl.
+
+End RegMachine.
+
+
+
+
+
 
